Proof of protocol-specific GetEpochAndConf on top of generic GetEpochAndConf

src/program_proof/simplepb/admin_proof.v
@@ -4,7 +4,7 @@ From Perennial.program_proof.grove_shared Require Import urpc_proof urpc_spec.
 From Perennial.goose_lang.lib Require Import waitgroup.
 From iris.base_logic Require Export lib.ghost_var mono_nat.
 From iris.algebra Require Import dfrac_agree mono_list.
-From Perennial.program_proof.simplepb Require Import pb_definitions.
+From Perennial.program_proof.simplepb Require Import pb_definitions config_proof.
 
 Section admin_proof.
 
@@ -21,6 +21,126 @@ Notation wp_Clerk__SetState := (wp_Clerk__SetState (pb_record:=pb_record)).
 
 Context `{!heapGS Σ}.
 Context `{!pbG Σ}.
+Context `{!configG Σ}.
+
+Definition adminN := nroot .@ "admin".
+
+Definition is_conf_inv γpb γconf : iProp Σ :=
+  inv adminN (∃ epoch conf (confγs:list pb_server_names) epoch_lb,
+      "Hepoch" ∷ own_epoch γconf epoch ∗
+      "Hconf" ∷ own_config γconf conf ∗
+      "#His_conf" ∷ is_epoch_config γpb epoch_lb confγs ∗
+      "#His_hosts" ∷ ([∗ list] γsrv ; host ∈ confγs ; conf, is_pb_host γpb γsrv host) ∗
+      "#His_lbs" ∷ (∀ γsrv, ⌜γsrv ∈ confγs⌝ → pb_ghost.is_epoch_lb γsrv epoch_lb) ∗
+      "Hunused" ∷ ([∗ set] epoch' ∈ (fin_to_set u64), ⌜int.nat epoch < int.nat epoch'⌝ → config_unset γpb epoch' ∗ config_unset γpb epoch') ∗
+      "Hunset" ∷ config_unset γpb epoch ∗
+      "#His_skip" ∷ (∀ epoch_skip, ⌜int.nat epoch_skip < int.nat epoch⌝ → ⌜int.nat epoch_lb < int.nat epoch_skip⌝ → is_epoch_skipped γpb epoch_skip)
+      )
+.
+
+Definition is_Clerk2 ck γpb : iProp Σ :=
+  ∃ γconf,
+    "#Hinv" ∷ is_conf_inv γpb γconf ∗
+    "#Hck" ∷ is_Clerk ck γconf.
+
+Lemma wp_Clerk__GetEpochAndConfig2 ck γpb Φ :
+  is_Clerk2 ck γpb -∗
+  □(∀ (epoch epoch_lb:u64) confγs (conf:list u64) config_sl,
+  (is_slice config_sl uint64T 1 conf ∗
+  config_unset γpb epoch ∗
+  is_epoch_config γpb epoch_lb confγs ∗
+  (∀ epoch_skip, ⌜int.nat epoch_skip < int.nat epoch⌝ → ⌜int.nat epoch_lb < int.nat epoch_skip⌝ → is_epoch_skipped γpb epoch_skip) ∗
+  ([∗ list] γsrv ; host ∈ confγs ; conf, is_pb_host γpb γsrv host) ∗
+  (∀ γsrv, ⌜γsrv ∈ confγs⌝ → pb_ghost.is_epoch_lb γsrv epoch_lb)) -∗
+   Φ (#epoch, slice_val config_sl)%V
+  ) -∗
+  WP config.Clerk__GetEpochAndConfig #ck {{ Φ }}
+.
+Proof.
+  iIntros "#Hck #HΦ".
+  iNamed "Hck".
+  wp_apply (wp_Clerk__GetEpochAndConfig with "[$Hck]").
+  iModIntro.
+  iIntros "Hlc".
+  iInv "Hinv" as "Hi" "Hclose".
+  iMod (lc_fupd_elim_later with "Hlc Hi") as "Hi".
+  iApply fupd_mask_intro.
+  { set_solver. }
+  iIntros "Hmask".
+  iNamed "Hi".
+  iExists _, _.
+  iFrame.
+  iIntros "%Hno_overflow Hepoch Hconf".
+  iMod "Hmask".
+
+  (* Hunset becomes skipped, and the first unused becomes unset. *)
+  iDestruct (big_sepS_elem_of_acc_impl (word.add epoch (U64 1)) with "Hunused") as "[Hunset_new Hunused]".
+  { set_solver. }
+  iMod (own_update with "Hunset") as "Hskip1".
+  {
+    apply singleton_update.
+    apply dfrac_agree_persist.
+  }
+  iDestruct "Hskip1" as "#Hskip1".
+  iSpecialize ("Hunset_new" with "[]").
+  { done. }
+  iDestruct "Hunset_new" as "[Hunset_new Hunset_new2]".
+
+  iMod ("Hclose" with "[Hunset_new2 Hunused Hepoch Hconf]").
+  {
+    iNext. iExists _, _, _, _.
+    iFrame "∗#".
+    iSplitL "Hunused".
+    {
+      iApply "Hunused".
+      {
+        iModIntro.
+        iIntros (???) "H". iIntros.
+        iApply "H".
+        iPureIntro.
+        word.
+      }
+      {
+        iIntros. exfalso. word.
+      }
+    }
+    iIntros (???).
+    assert (int.nat epoch_skip = int.nat epoch ∨ int.nat epoch_skip < int.nat epoch ∨ int.nat epoch_skip >= int.nat (word.add epoch (U64 1))) as Hineq.
+    { word. }
+    destruct Hineq as [Heq|[Hineq|Hineq]].
+    {
+      replace (epoch_skip) with (epoch) by word.
+      iFrame "Hskip1".
+    }
+    {
+      iApply "His_skip".
+      { done. }
+      { done. }
+    }
+    { exfalso. word. }
+  }
+  iModIntro.
+  iIntros.
+  iApply "HΦ".
+  iFrame "∗#".
+
+  (* TODO: repetetive proof *)
+  iIntros.
+  assert (int.nat epoch_skip = int.nat epoch ∨ int.nat epoch_skip < int.nat epoch ∨ int.nat epoch_skip >= int.nat (word.add epoch (U64 1))) as Hineq.
+  { word. }
+  destruct Hineq as [Heq|[Hineq|Hineq]].
+  {
+    replace (epoch_skip) with (epoch) by word.
+    iFrame "Hskip1".
+  }
+  {
+    iApply "His_skip".
+    { done. }
+    { done. }
+  }
+  { exfalso. word. }
+Qed.
+
 Lemma wp_Reconfig γ (configHost:u64) (servers:list u64) (servers_sl:Slice.t) :
   {{{
         "Hservers_sl" ∷ is_slice servers_sl uint64T 1 servers ∗
@@ -34,4 +154,8 @@ Proof.
   iIntros (Φ) "Hpre HΦ".
   iNamed "Hpre".
   wp_call.
+  wp_apply (wp_MakeClerk with "").
+  { admit. }
 Admitted.
+
+End admin_proof.
